Rename InstComplete -> Closed

src/ReactorModel/Execution/Basic.lean
@@ -86,13 +86,15 @@ def InstExecution.rcns (e : s₁ ⇓ᵢ+ s₂) : List ID :=
 def InstExecution.changes (e : s₁ ⇓ᵢ+ s₂) : List (Identified Change) :=
   e.ops.map (·.changes) |>.join
 
-abbrev State.InstComplete (s : State) : Prop := s.ctx.currentProcessedRcns = s.rtr.ids .rcn
+abbrev State.Closed (s : State) : Prop := s.ctx.currentProcessedRcns = s.rtr.ids .rcn
 
-theorem State.InstComplete.processedRcns_not_empty : InstComplete s → s.ctx.processedRcns ≠ ∅ := 
+theorem State.Closed.processedRcns_not_empty : Closed s → s.ctx.processedRcns ≠ ∅ := 
   sorry  
 
+open State (Closed)
+
 inductive CompleteInstExecution (s₁ s₂ : State) : Prop
-  | mk (exec : s₁ ⇓ᵢ+ s₂) (complete : s₂.InstComplete)
+  | mk (exec : s₁ ⇓ᵢ+ s₂) (closed : Closed s₂)
   
 notation s₁:max " ⇓ᵢ| " s₂:max => CompleteInstExecution s₁ s₂
 
@@ -101,7 +103,7 @@ theorem clearingPorts_unique : clearingPorts σ σ₁ → clearingPorts σ σ₂
 
 inductive AdvanceTag : State → State → Prop 
   | mk (hg : s.nextTag = some g) : 
-    (s.InstComplete) →
+    (Closed s) →
     (clearingPorts s.rtr σ) →
     AdvanceTag s ⟨σ, s.ctx.advanceTag g $ s.tag_lt_nextTag hg⟩
 
@@ -110,8 +112,8 @@ notation s₁:max " ⇓ₜ " s₂:max => AdvanceTag s₁ s₂
 -- Now we define a fully timed step, which can be a full instaneous execution, i.e. until no more
 -- steps can be taken, or a time advancement.
 inductive Step (s₁ s₂ : State) : Prop 
-  | completeInst (h : s₁ ⇓ᵢ| s₂)
-  | advanceTag (h : s₁ ⇓ₜ s₂)
+  | close (h : s₁ ⇓ᵢ| s₂)
+  | advance (h : s₁ ⇓ₜ s₂)
 
 notation s₁:max " ⇓ " s₂:max => Step s₁ s₂
 
