src/ReactorModel/Determinism/ExecutionStep.lean
@@ -2,18 +2,18 @@ import ReactorModel.Determinism.InstExecution
 
 namespace Execution
 
-open State (InstComplete)
+open State (Closed)
 
-theorem AdvanceTag.instComplete : (s₁ ⇓ₜ s₂) → InstComplete s₁
+theorem AdvanceTag.closed : (s₁ ⇓ₜ s₂) → Closed s₁
   | mk _ h _ => h
 
-theorem AdvanceTag.not_InstComplete : (s₁ ⇓ₜ s₂) → ¬(InstComplete s₂)
+theorem AdvanceTag.not_Closed : (s₁ ⇓ₜ s₂) → ¬(Closed s₂)
   | mk hg _ _, h => by
     have h' := s₁.ctx.advanceTag_processedRcns_empty $ s₁.tag_lt_nextTag hg
     exact absurd h' h.processedRcns_not_empty
 
-theorem AdvanceTag.saturating (a₁ : s₁ ⇓ₜ s₂) (a₂ : s₂ ⇓ₜ s₃) : False :=
-  absurd a₂.instComplete a₁.not_InstComplete
+theorem AdvanceTag.nonrepeatable (a : s₁ ⇓ₜ s₂) : ¬(s₂ ⇓ₜ s₃) :=
+  (absurd ·.closed a.not_Closed)
 
 theorem AdvanceTag.tag_lt : (s₁ ⇓ₜ s₂) → s₁.ctx.tag < s₂.ctx.tag
   | mk .. => by simp [Context.advanceTag_strictly_increasing]
@@ -23,18 +23,18 @@ theorem AdvanceTag.determinisic : (s ⇓ₜ s₁) → (s ⇓ₜ s₂) → s₁ =
     simp only [hg₁, Option.some_inj] at hg₂
     simp [clearingPorts_unique hc₁ hc₂, Context.advanceTag, hg₂]  
 
-theorem CompleteInstExecution.complete : (s₁ ⇓ᵢ| s₂) → InstComplete s₂
+theorem CompleteInstExecution.closed : (s₁ ⇓ᵢ| s₂) → Closed s₂
   | mk _ h => h
 
-theorem CompleteInstExecution.not_InstComplete : (s₁ ⇓ᵢ| s₂) → ¬(InstComplete s₁)
-  | mk e _ => e.not_InstComplete
+theorem CompleteInstExecution.not_Closed : (s₁ ⇓ᵢ| s₂) → ¬(Closed s₁)
+  | mk e _ => e.not_Closed
 
-theorem CompleteInstExecution.saturating (e₁ : s₁ ⇓ᵢ| s₂) (e₂ : s₂ ⇓ᵢ| s₃) : False :=
-  absurd e₁.complete e₂.not_InstComplete
+theorem CompleteInstExecution.nonrepeatable (e : s₁ ⇓ᵢ| s₂) : ¬(s₂ ⇓ᵢ| s₃) :=
+  (absurd e.closed ·.not_Closed)
 
-theorem CompleteInstExecution.currentProcessedRcns_monotonic :
+theorem CompleteInstExecution.currentProcessedRcns_ssubset :
   (s₁ ⇓ᵢ| s₂) → s₁.ctx.currentProcessedRcns ⊂ s₂.ctx.currentProcessedRcns
-  | mk exec _ => exec.currentProcessedRcns_monotonic
+  | mk e _ => e.currentProcessedRcns_ssubset
 
 theorem CompleteInstExecution.rcns_eq : (s ⇓ᵢ| s₁) → (s ⇓ᵢ| s₂) → s₁.rtr.ids .rcn = s₂.rtr.ids .rcn
   | mk e₁ _, mk e₂ _ => by 
@@ -65,21 +65,21 @@ theorem CompleteInstExecution.deterministic : (s ⇓ᵢ| s₁) → (s ⇓ᵢ| s�
   | i₁@(mk e₁ _), i₂@(mk e₂ _) => e₁.deterministic e₂ $ i₁.convergent_ctx i₂
 
 theorem CompleteInstExecution.not_AdvanceTag : (s ⇓ᵢ| s₁) → ¬(s ⇓ₜ s₂) := 
-  fun ⟨e, _⟩ ⟨_, h, _⟩ => absurd h e.not_InstComplete
+  fun ⟨e, _⟩ ⟨_, h, _⟩ => absurd h e.not_Closed
 
 theorem Step.tag_le : (s₁ ⇓ s₂) → s₁.ctx.tag ≤ s₂.ctx.tag
-  | completeInst e => le_of_eq e.tag_eq
-  | advanceTag a   => le_of_lt a.tag_lt
+  | close e   => le_of_eq e.tag_eq
+  | advance a => le_of_lt a.tag_lt
 
 protected theorem Step.deterministic : (s ⇓ s₁) → (s ⇓ s₂) → s₁ = s₂
-  | completeInst e₁, completeInst e₂                            => e₁.deterministic e₂
-  | advanceTag a₁, advanceTag a₂                                => a₁.determinisic a₂
-  | completeInst e, advanceTag a | advanceTag a, completeInst e => absurd a e.not_AdvanceTag
+  | close e₁, close e₂                      => e₁.deterministic e₂
+  | advance a₁, advance a₂                  => a₁.determinisic a₂
+  | close e, advance a | advance a, close e => absurd a e.not_AdvanceTag
 
 theorem Step.seq_tag_lt : (s₁ ⇓ s₂) → (s₂ ⇓ s₃) → s₁.ctx.tag < s₃.ctx.tag
-  | advanceTag a₁,   advanceTag a₂   => False.elim $ a₁.saturating a₂
-  | completeInst e₁, completeInst e₂ => False.elim $ e₁.saturating e₂
-  | advanceTag a,    completeInst e  => e.tag_eq ▸ a.tag_lt
-  | completeInst e,  advanceTag a    => e.tag_eq ▸ a.tag_lt
+  | advance a₁, advance a₂ => absurd a₂ a₁.nonrepeatable 
+  | close e₁,   close e₂   => absurd e₂ e₁.nonrepeatable
+  | advance a,  close e    => e.tag_eq ▸ a.tag_lt
+  | close e,    advance a  => e.tag_eq ▸ a.tag_lt
 
 end Execution
